FlatMemory.thy
@@ -1,0 +1,63 @@
+theory FlatMemory
+  imports HeapMemory
+begin
+
+datatype flat_state = 
+  FS "nat heap" "ptr list" "ptr list list" "nat list" (code: "byte_code list")
+
+fun get_closure :: "nat heap \<Rightarrow> nat \<Rightarrow> hclosure" where
+  "get_closure h p = (case hlookup h p of
+      0 \<Rightarrow> HConst (hlookup h (Suc p))
+    | Suc x \<Rightarrow> HLam (hlookup_list h (Suc (Suc p)) x) (hlookup h (Suc p)))"
+
+inductive evalf :: "flat_state \<Rightarrow> flat_state \<Rightarrow> bool" (infix "\<leadsto>\<^sub>f" 50) where
+  evf_lookup [simp]: "cd ! pc = BLookup x \<Longrightarrow> lookup env x = Some v \<Longrightarrow> 
+    FS h vs (env # envs) (Suc pc # pcs) cd \<leadsto>\<^sub>f FS h (v # vs) envs (pc # pcs) cd"
+| evf_pushcon [simp]: "cd ! pc = BPushCon k \<Longrightarrow> halloc_list h [0, k] = (h', v) \<Longrightarrow>
+    FS h vs (env # envs) (Suc pc # pcs) cd \<leadsto>\<^sub>f FS h' (v # vs) envs (pc # pcs) cd"
+| evf_pushlam [simp]: "cd ! pc = BPushLam pc' \<Longrightarrow> 
+    halloc_list h (Suc (length env) # pc' # env) = (h', v) \<Longrightarrow>
+      FS h vs (env # envs) (Suc pc # pcs) cd \<leadsto>\<^sub>f FS h' (v # vs) envs (pc # pcs) cd"
+| evf_enter [simp]: "cd ! pc = BEnter \<Longrightarrow> 
+    FS h vs (env # envs) (Suc pc # pcs) cd \<leadsto>\<^sub>f FS h vs (env # env # envs) (pc # pcs) cd"
+| evf_apply [simp]: "cd ! pc = BApply \<Longrightarrow> get_closure h v2 = HLam env pc' \<Longrightarrow>
+    FS h (v1 # v2 # vs) envs (Suc pc # pcs) cd \<leadsto>\<^sub>f
+      FS h vs ((v1 # env) # envs) (pc' # pc # pcs) cd"
+| evf_return [simp]: "cd ! pc = BReturn \<Longrightarrow> 
+    FS h vs envs (Suc pc # pcs) cd \<leadsto>\<^sub>f FS h vs envs pcs cd"
+
+theorem determinismf: "\<Sigma> \<leadsto>\<^sub>f \<Sigma>' \<Longrightarrow> \<Sigma> \<leadsto>\<^sub>f \<Sigma>'' \<Longrightarrow> \<Sigma>' = \<Sigma>''"
+proof (induction \<Sigma> \<Sigma>' rule: evalf.induct)
+  case (evf_lookup cd pc x env v h vs envs pcs)
+  from evf_lookup(3, 1, 2) show ?case 
+    by (induction "FS h vs (env # envs) (Suc pc # pcs) cd" \<Sigma>'' rule: evalf.induct) simp_all 
+next
+  case (evf_pushcon cd pc k h h' v vs env envs pcs)
+  from evf_pushcon(3, 1, 2) show ?case 
+    by (induction "FS h vs (env # envs) (Suc pc # pcs) cd" \<Sigma>'' rule: evalf.induct) simp_all 
+next
+  case (evf_pushlam cd pc pc' h env h' v vs envs pcs)
+  from evf_pushlam(3, 1, 2) show ?case 
+    by (induction "FS h vs (env # envs) (Suc pc # pcs) cd" \<Sigma>'' rule: evalf.induct) simp_all 
+next
+  case (evf_enter cd pc h vs env envs pcs)
+  from evf_enter(2, 1) show ?case 
+    by (induction "FS h vs (env # envs) (Suc pc # pcs) cd" \<Sigma>'' rule: evalf.induct) simp_all 
+next
+  case (evf_apply cd pc h v2 env pc' v1 vs envs pcs)
+  from evf_apply(3, 1, 2) show ?case 
+    by (induction "FS h (v1 # v2 # vs) envs (Suc pc # pcs) cd" \<Sigma>'' rule: evalf.induct) 
+       simp_all 
+next
+  case (evf_return cd pc h vs envs pcs)
+  from evf_return(2, 1) show ?case 
+    by (induction "FS h vs envs (Suc pc # pcs) cd" \<Sigma>'' rule: evalf.induct) simp_all 
+qed
+
+lemma [simp]: "\<Sigma> \<leadsto>\<^sub>f \<Sigma>' \<Longrightarrow> code \<Sigma> = code \<Sigma>'"
+  by (induction \<Sigma> \<Sigma>' rule: evalf.induct) simp_all
+
+lemma [simp]: "iter (\<leadsto>\<^sub>f) \<Sigma> \<Sigma>' \<Longrightarrow> code \<Sigma> = code \<Sigma>'"
+  by (induction \<Sigma> \<Sigma>' rule: iter.induct) simp_all
+
+end
